Extend CRpower to N (from positive) and make an instance of Pow.

reals/fast/CRpower.v
@@ -32,39 +32,40 @@ Open Local Scope Q_scope.
 Open Local Scope uc_scope.
 
 (**
-** Positive Integer Powers
+** Natural Integer Powers
 Positive integer powers is faster than repeated multiplication.
 
 It is uniformly continuous on an interval [[-c,c]].
 *)
-Section CRpower_positive.
+Section CRpower_N.
 
-Variable p: positive.
+Variable n : N.
 
-Definition Qpower_positive_modulus (c:Qpos) (e:Qpos) : QposInf :=
-Qpos2QposInf (e/((p#1)*c^(Zpred p))).
+Definition Qpower_N_modulus (c:Qpos) (e:Qpos) : QposInf :=
+  match n with 
+  | N0 => QposInfinity
+  | Npos p => Qpos2QposInf (e/((p#1)*c^(Zpred p)))
+  end.
 
 Lemma Qpower_positive_correct : forall p q, (inj_Q IR (Qpower_positive q p)[=]((FId{^}(nat_of_P p)) (inj_Q IR q) I)).
 Proof.
- clear p.
  intros p.
- destruct (p_is_some_anti_convert p) as [n Hn].
+ destruct (p_is_some_anti_convert p) as [m Hm].
  simpl.
- rewrite Hn.
- clear Hn.
+ subst.
  intros q.
- induction n.
+ induction m.
   simpl.
   algebra.
  rewrite nat_of_P_o_P_of_succ_nat_eq_succ.
- rewrite nat_of_P_o_P_of_succ_nat_eq_succ in IHn.
- change (P_of_succ_nat (S n)) with (Psucc (P_of_succ_nat n)).
+ rewrite nat_of_P_o_P_of_succ_nat_eq_succ in IHm.
+ change (P_of_succ_nat (S m)) with (Psucc (P_of_succ_nat m)).
  simpl in *.
  rewrite Pplus_one_succ_r.
- stepl (inj_Q IR (Qpower_positive q (P_of_succ_nat n))[*](inj_Q IR q)).
-  csetoid_rewrite IHn.
+ stepl (inj_Q IR (Qpower_positive q (P_of_succ_nat m))[*](inj_Q IR q)).
+  csetoid_rewrite IHm.
   apply eq_reflexive.
- stepl (inj_Q IR (Qpower_positive q (P_of_succ_nat n)*q)).
+ stepl (inj_Q IR (Qpower_positive q (P_of_succ_nat m)*q)).
   apply inj_Q_wd.
   simpl.
   rewrite -> Qpower_plus_positive.
@@ -72,12 +73,16 @@ Proof.
  apply inj_Q_mult.
 Qed.
 
-Let IRpower_p : PartFunct IR := FId{^}(nat_of_P p).
+Let IRpower_p : PartFunct IR := FId{^}(nat_of_N n).
 
-Lemma Qpower_positive_uc_prf (c:Qpos) :  is_UniformlyContinuousFunction (fun x => Qpower_positive (QboundAbs c x) p) (Qpower_positive_modulus c).
+Lemma Qpower_N_uc_prf (c:Qpos) : 
+  is_UniformlyContinuousFunction (fun x => Qpower (QboundAbs c x) (Z_of_N n)) (Qpower_N_modulus c).
 Proof.
- destruct (p_is_some_anti_convert p) as [n Hn].
- assert (X:=(fun I pI => Derivative_nth I pI _ _ (Derivative_id I pI) n)).
+ unfold Qpower_N_modulus.
+ destruct n as [|p].
+  simpl. intros e x y E. now apply ball_refl.
+ destruct (p_is_some_anti_convert p) as [m Hm].
+ assert (X:=(fun I pI => Derivative_nth I pI _ _ (Derivative_id I pI) m)).
  assert (-c < c)%Q.
   rewrite -> Qlt_minus_iff.
   ring_simplify.
@@ -86,7 +91,6 @@ Proof.
  apply (fun x => @is_UniformlyContinuousFunction_wd _ _ (fun x : Q_as_MetricSpace => Qpower_positive (QboundAbs c x) p) x (Qscale_modulus ((p#1)*c^(Zpred p))%Qpos)).
    reflexivity.
   intros x.
-  unfold Qpower_positive_modulus.
   generalize ((p # 1) * c ^ Zpred p)%Qpos.
   apply Qpos_positive_numerator_rect.
   intros qn qd.
@@ -99,44 +103,44 @@ Proof.
   intros q _ Hq.
   csetoid_rewrite (Qpower_positive_correct p q).
   simpl.
-  rewrite Hn.
+  rewrite Hm.
   simpl.
   rewrite nat_of_P_o_P_of_succ_nat_eq_succ.
   apply eq_reflexive.
  simpl.
  intros x _ Hx.
- change (AbsIR ((nring (R:=IR) (S n))[*](One[*]nexp IR n (inj_Q IR x)))[<=]
+ change (AbsIR ((nring (R:=IR) (S m))[*](One[*]nexp IR m (inj_Q IR x)))[<=]
    inj_Q IR (((p # 1)[*]((c ^ Zpred p)%Qpos:Q)))).
  stepr ((inj_Q IR ((p # 1))[*](inj_Q IR ((c ^ Zpred p)%Qpos:Q)))); [| now
    (apply eq_symmetric; apply inj_Q_mult)].
- stepl ((nring (R:=IR) (S n)[*]AbsIR (One[*]nexp IR n (inj_Q IR x)))); [| now apply AbsIR_mult;apply nring_nonneg; auto with *].
+ stepl ((nring (R:=IR) (S m)[*]AbsIR (One[*]nexp IR m (inj_Q IR x)))); [| now apply AbsIR_mult;apply nring_nonneg; auto with *].
  apply mult_resp_leEq_both.
     apply nring_nonneg; auto with *.
    apply AbsIR_nonneg.
-  stepl (inj_Q IR (nring (S n))); [| now apply inj_Q_nring].
+  stepl (inj_Q IR (nring (S m))); [| now apply inj_Q_nring].
   apply inj_Q_leEq.
-  rewrite Hn.
+  rewrite Hm.
   rewrite <- POS_anti_convert.
-  stepl ((S n):Q); [| now apply eq_symmetric; apply nring_Q].
+  stepl ((S m):Q); [| now apply eq_symmetric; apply nring_Q].
   apply leEq_reflexive.
- stepl (One[*](AbsIR (nexp IR n (inj_Q IR x)))); [| now apply AbsIR_mult; apply less_leEq; apply pos_one].
- stepl (AbsIR (nexp IR n (inj_Q _ x))); [| now apply eq_symmetric; apply one_mult].
- stepl (nexp IR n (AbsIR (inj_Q _ x))); [| now apply eq_symmetric; apply AbsIR_nexp].
+ stepl (One[*](AbsIR (nexp IR m (inj_Q IR x)))); [| now apply AbsIR_mult; apply less_leEq; apply pos_one].
+ stepl (AbsIR (nexp IR m (inj_Q _ x))); [| now apply eq_symmetric; apply one_mult].
+ stepl (nexp IR m (AbsIR (inj_Q _ x))); [| now apply eq_symmetric; apply AbsIR_nexp].
  stepr (inj_Q IR (c ^ Zpred p)); [| now apply inj_Q_wd; reflexivity].
- rewrite Hn.
+ rewrite Hm.
  rewrite <- POS_anti_convert.
  rewrite inj_S.
  rewrite <- Zpred_succ.
- destruct n.
+ destruct m.
   change (One[<=]inj_Q IR (nring 1)).
   stepr (nring (R:=IR) 1); [| now apply eq_symmetric; apply inj_Q_nring].
   stepr (One:IR).
    apply leEq_reflexive.
   simpl; algebra.
- rewrite  <- (nat_of_P_o_P_of_succ_nat_eq_succ n).
+ rewrite  <- (nat_of_P_o_P_of_succ_nat_eq_succ m).
  rewrite convert_is_POS.
  simpl.
- stepr ((FId{^}(nat_of_P (P_of_succ_nat n))) (inj_Q IR (c:Q)) I); [| now apply eq_symmetric; apply Qpower_positive_correct].
+ stepr ((FId{^}(nat_of_P (P_of_succ_nat m))) (inj_Q IR (c:Q)) I); [| now apply eq_symmetric; apply Qpower_positive_correct].
  simpl.
  apply: power_resp_leEq.
   apply AbsIR_nonneg.
@@ -147,14 +151,15 @@ Proof.
  apply inj_Q_inv.
 Qed.
 
-Definition Qpower_positive_uc (c:Qpos) :  Q_as_MetricSpace --> Q_as_MetricSpace :=
-Build_UniformlyContinuousFunction (Qpower_positive_uc_prf c).
+Definition Qpower_N_uc (c:Qpos) :  Q_as_MetricSpace --> Q_as_MetricSpace :=
+Build_UniformlyContinuousFunction (Qpower_N_uc_prf c).
 
 (** CRpower_positive_bounded works on [[-c,c]]. *)
-Definition CRpower_positive_bounded (c:Qpos) : CR --> CR :=
-Cmap QPrelengthSpace (Qpower_positive_uc c).
+Definition CRpower_N_bounded (c:Qpos) : CR --> CR :=
+Cmap QPrelengthSpace (Qpower_N_uc c).
 
-Lemma CRpower_positive_bounded_correct : forall (c:Qpos) x, AbsSmall (inj_Q _ (c:Q)) x -> (IRasCR (x[^](nat_of_P p))==CRpower_positive_bounded c (IRasCR x))%CR.
+Lemma CRpower_N_bounded_correct : forall (c:Qpos) x, 
+  AbsSmall (inj_Q _ (c:Q)) x -> (IRasCR (x[^](nat_of_N n))==CRpower_N_bounded c (IRasCR x))%CR.
 Proof.
  intros c x Hx.
  pose (I:=(clcr [--](inj_Q IR (c:Q)) (inj_Q IR (c:Q)))).
@@ -169,12 +174,12 @@ Proof.
   rstepr (inj_Q IR (c:Q)[+]inj_Q IR (c:Q)).
   apply plus_resp_pos; assumption.
  rename I into temp.
- change (x[^](nat_of_P p)) with ((FId{^}(nat_of_P p)) x True_constr).
+ change (x[^](nat_of_N n)) with ((FId{^}(nat_of_N n)) x True_constr).
  rename temp into I.
  destruct Hx as [Hx0 Hx1].
- apply (ContinuousCorrect HI (Continuous_nth I FId (Continuous_id I)  (nat_of_P p)));[|split;assumption].
+ apply (ContinuousCorrect HI (Continuous_nth I FId (Continuous_id I)  (nat_of_N n)));[|split;assumption].
  intros q [] Hq.
- transitivity (IRasCR (inj_Q IR (Qpower_positive q p))).
+ transitivity (IRasCR (inj_Q IR (Qpower q (Z_of_N n)))).
   rewrite -> IR_inj_Q_as_CR.
   simpl.
   change (' q)%CR with (Cunit_fun _ q).
@@ -193,24 +198,26 @@ Proof.
   apply leEq_inj_Q with IR.
   destruct Hq; assumption.
  apply IRasCR_wd.
- apply Qpower_positive_correct.
+ destruct n.
+  simpl. now apply inj_Q_One.
+ simpl. now apply Qpower_positive_correct.
 Qed.
 
-Lemma CRpower_positive_bounded_weaken : forall (c1 c2:Qpos) x,
+Lemma CRpower_N_bounded_weaken : forall (c1 c2:Qpos) x,
 ((AbsSmall ('c1) x) -> (c1 <= c2)%Q ->
-CRpower_positive_bounded c1 x == CRpower_positive_bounded c2 x)%CR.
+CRpower_N_bounded c1 x == CRpower_N_bounded c2 x)%CR.
 Proof.
  intros c1 c2 x Hx Hc.
  simpl in x.
  rewrite <- (CRasIRasCR_id x).
- transitivity (IRasCR ((CRasIR x)[^](nat_of_P p))).
+ transitivity (IRasCR ((CRasIR x)[^](nat_of_N n))).
   symmetry.
-  apply CRpower_positive_bounded_correct.
+  apply CRpower_N_bounded_correct.
   rewrite -> IR_AbsSmall_as_CR.
   stepl ('c1)%CR; [| now simpl; symmetry; apply IR_inj_Q_as_CR].
   stepr x; [| now simpl; symmetry; apply CRasIRasCR_id].
   assumption.
- apply CRpower_positive_bounded_correct.
+ apply CRpower_N_bounded_correct.
  apply AbsSmall_leEq_trans with (inj_Q IR (c1:Q)).
   apply inj_Q_leEq.
   assumption.
@@ -222,11 +229,11 @@ Qed.
 
 (** [CRpower_positive_bounded] is should be used when a known bound
 on the absolute value of x is available. *)
-Definition CRpower_positive (x:CR) : CR := ucFun (CRpower_positive_bounded (CR_b (1#1) x)) x.
+Definition CRpower_N (x:CR) : CR := ucFun (CRpower_N_bounded (CR_b (1#1) x)) x.
 
-Lemma CRpositive_power_bounded_positive_power : forall (c:Qpos) (x:CR),
+Lemma CRpower_N_bounded_N_power : forall (c:Qpos) (x:CR),
 ((AbsSmall ('c) x) ->
-CRpower_positive_bounded c x == CRpower_positive x)%CR.
+CRpower_N_bounded c x == CRpower_N x)%CR.
 Proof.
  intros c x Hc.
  assert (Hx:(AbsSmall ('(CR_b (1#1) x)) x)%CR).
@@ -234,17 +241,17 @@ Proof.
    rewrite -> CRopp_Qopp.
    apply CR_b_lowerBound.
   apply CR_b_upperBound.
- unfold CRpower_positive.
+ unfold CRpower_N.
  generalize (CR_b (1#1) x) Hx.
  clear Hx.
  intros d Hd.
- destruct (Qle_total c d);[|symmetry]; apply CRpower_positive_bounded_weaken; assumption.
+ destruct (Qle_total c d);[|symmetry]; apply CRpower_N_bounded_weaken; assumption.
 Qed.
 
-Lemma CRpower_positive_correct : forall x, (IRasCR (x[^](nat_of_P p))==CRpower_positive (IRasCR x))%CR.
+Lemma CRpower_N_correct : forall x, (IRasCR (x[^](nat_of_N n))==CRpower_N (IRasCR x))%CR.
 Proof.
  intros x.
- apply CRpower_positive_bounded_correct.
+ apply CRpower_N_bounded_correct.
  rewrite -> IR_AbsSmall_as_CR.
  stepl ('(CR_b (1#1) (IRasCR x)))%CR; [| now simpl; symmetry; apply IR_inj_Q_as_CR].
  split.
@@ -253,38 +260,37 @@ Proof.
  apply CR_b_upperBound.
 Qed.
 
-End CRpower_positive.
+End CRpower_N.
 
-Lemma CRpower_positive_correct' : forall n x,
-(IRasCR (x[^]S n)==CRpower_positive (P_of_succ_nat n) (IRasCR x))%CR.
+Lemma CRpower_N_correct' : forall n x,
+(IRasCR (x[^]n)==CRpower_N (N_of_nat n) (IRasCR x))%CR.
 Proof.
  intros n x.
- rewrite <- nat_of_P_o_P_of_succ_nat_eq_succ.
- apply CRpower_positive_correct.
+ etransitivity; [| apply CRpower_N_correct].
+ now rewrite Nnat.nat_of_N_of_nat.
 Qed.
 
-Hint Rewrite CRpower_positive_correct' : IRtoCR.
+Hint Rewrite CRpower_N_correct' : IRtoCR.
 
-Instance: Proper (eq ==> QposEq ==> @st_eq _) Qpower_positive_uc.
+Instance: Proper (eq ==> QposEq ==> @st_eq _) Qpower_N_uc.
 Proof.
  intros p1 p2 Ep e1 e2 Ee x.
  apply ball_eq_iff. intro e.
  simpl. unfold QposEq in Ee. rewrite Ep, Ee. reflexivity.
 Qed.
 
-Instance: Proper (eq ==> QposEq ==> @st_eq _) CRpower_positive_bounded. 
+Instance: Proper (eq ==> QposEq ==> @st_eq _) CRpower_N_bounded. 
 Proof. 
  intros p1 p2 Ep e1 e2 Ee x. simpl. rewrite Ep, Ee. reflexivity.
 Qed. 
 
-(* begin hide *)
-Add Parametric Morphism p : (@CRpower_positive p) with signature (@st_eq _) ==> (@st_eq _) as CRpower_positive_wd.
+Instance: Proper (eq ==> @st_eq _ ==> @st_eq _) CRpower_N.
 Proof.
- intros x1 x2 Hx.
- transitivity (CRpower_positive_bounded p (CR_b (1 # 1) x1) x2).
-  change (ucFun (CRpower_positive_bounded p (CR_b (1#1) x1)) x1==ucFun (CRpower_positive_bounded p (CR_b (1#1) x1)) x2)%CR.
+ intros ? n Hn x1 x2 Hx. subst.
+ transitivity (CRpower_N_bounded n (CR_b (1 # 1) x1) x2).
+  change (ucFun (CRpower_N_bounded n (CR_b (1#1) x1)) x1==ucFun (CRpower_N_bounded n (CR_b (1#1) x1)) x2)%CR.
   apply uc_wd; assumption.
- apply CRpositive_power_bounded_positive_power.
+ apply CRpower_N_bounded_N_power.
  split; rewrite <- Hx.
   rewrite -> CRopp_Qopp.
   apply CR_b_lowerBound.
